theories/iris/rules/iris_rules_exceptions.v
@@ -1,0 +1,699 @@
+
+From iris.proofmode Require Import base tactics classes.
+From iris.program_logic Require Import weakestpre.
+From Wasm.iris.language Require Import iris_ewp_ctx.
+From Wasm.iris.helpers Require Import iris_properties.
+From stdpp Require Import base list.
+From mathcomp Require Import ssreflect eqtype seq ssrbool.
+
+
+
+
+
+Set Bullet Behavior "Strict Subproofs".
+Close Scope byte_scope.
+
+
+(* ========================================================================== *)
+(** * Reasoning Rules. *)
+
+Section reasoning_rules.
+  Context `{!wasmG Σ}.
+
+   Lemma tag_valid gm a tf:
+    gen_heap_interp gm -∗ a ↦□[tag] tf -∗ ⌜ gm !! a = Some tf ⌝.
+  Proof.
+    iIntros "Htags Htag".
+    iDestruct (gen_heap_valid with "Htags Htag") as "%Htag".
+    done.
+  Qed. 
+
+  Lemma ewp_throw f x a ves vcs ts E Ψ Φ:
+    List.nth_error (inst_tags (f_inst f)) x = Some a ->
+    ves = v_to_e_list vcs ->
+    length ves = length ts ->
+    N.of_nat a ↦□[tag] (Tf ts []) ∗
+      ▷ (∀ i, N.of_nat i ↦[we] {| e_tag := Mk_tagidx a ; e_fields := vcs |} -∗
+             EWP [AI_ref_exn i (Mk_tagidx a); AI_basic BI_throw_ref] UNDER f @ E <| Ψ |> {{ Φ }})
+      ⊢ EWP ves ++ [AI_basic (BI_throw x)] UNDER f @ E <| Ψ |> {{ Φ }}.
+  Proof.
+    iIntros (Hx -> Hlen) "[#Htag Hwp]".
+    iApply ewp_lift_step.
+    { rewrite to_val_cat_None2 => //.
+      apply v_to_e_is_const_list. }
+    { rewrite to_eff_cat_None2 => //.
+      apply v_to_e_is_const_list. }
+    iIntros (σ) "Hσ".
+    iApply fupd_mask_intro; first solve_ndisj.
+    iIntros "Hclose".
+
+    iDestruct "Hσ" as "(Hfuncs & Hconts & Hexns & Htags & Hrest)".
+    iDestruct (tag_valid with "Htags Htag") as "%Htag".
+    rewrite gmap_of_list_lookup in Htag.
+    rewrite Nat2N.id in Htag.
+    iSplit.
+    { iPureIntro.
+      eexists _,(_,_),_,_.
+      repeat split => //.
+      eapply r_throw => //.
+      exact Hx.
+      rewrite nth_error_lookup //.
+      exact Htag.
+      done.
+    }
+    iIntros "!>" (e2 ?? HStep).
+    iMod (gen_heap_alloc with "Hexns") as "(Hexns & Hexn & Htok)"; last first. 
+    iMod "Hclose".
+    iModIntro.
+
+    destruct HStep as (Hred & _).
+    edestruct reduce_det.
+    exact Hred.
+    eapply r_throw => //; eauto.
+    rewrite nth_error_lookup //.
+    destruct H0.
+    - destruct H0 as [-> ->].
+      subst f. 
+      iFrame "Hfuncs Hconts Htags Hrest".
+      iSplitR "Hwp Hexn"; last first.
+      + iApply ("Hwp" with "Hexn").
+      + unfold add_exn. simpl.
+        rewrite -gmap_of_list_append.
+        iFrame. 
+    - destruct H0 as [[? H'] | (? & ? & ? & H' & _)].
+      all: rewrite first_instr_const in H' => //.
+      all: apply v_to_e_is_const_list.
+    - rewrite gmap_of_list_lookup.
+      rewrite Nat2N.id.
+      apply lookup_ge_None_2.
+      lia.
+  Qed. 
+
+  Lemma ewp_throw_ref a exn i Ψ f E Φ:
+    i = e_tag exn ->
+    N.of_nat a ↦[we] exn ∗ get_throw i Ψ (e_fields exn) a
+      ⊢ EWP [AI_ref_exn a i; AI_basic BI_throw_ref] UNDER f @ E <| Ψ |> {{ Φ }}.
+  Proof.
+    iIntros (->) "[Hexn HΨ]".
+    iApply ewp_lift_step => //.
+    iIntros (σ) "Hσ".
+    iApply fupd_mask_intro; first solve_ndisj.
+    iIntros "Hclose".
+
+    iDestruct "Hσ" as "(Hfuncs & Hconts & Hexns & Hrest)".
+    iDestruct (gen_heap_valid with "Hexns Hexn") as %Hexn.
+    rewrite gmap_of_list_lookup in Hexn.
+    rewrite Nat2N.id in Hexn.
+    iSplit.
+    { iPureIntro.
+      eexists _,(_,_),_,_.
+      repeat split => //.
+      eapply r_throw_ref_desugar => //.
+      rewrite nth_error_lookup //.
+    }
+    iIntros "!>" (e2 ?? HStep).
+    iMod "Hclose".
+    iModIntro.
+
+    destruct HStep as (Hred & _).
+    edestruct reduce_det.
+    exact Hred.
+    eapply r_throw_ref_desugar => //; eauto.
+    rewrite nth_error_lookup //.
+    destruct H0.
+    - destruct H0 as [-> ->].
+      subst f. 
+      iFrame.
+      iApply ewp_effect_thr => //. 
+    - destruct H0 as [[? H'] | (? & ? & ? & H' & _)].
+      done. done.
+  Qed.
+
+  Definition agree_on_uncaptured decs (Ψ Ψ' : meta_protocol) : Prop :=
+    (forall i, get_suspend i Ψ = get_suspend i Ψ') /\
+      (forall i, get_switch i Ψ = get_switch i Ψ') /\
+      (forall i, firstx_exception decs i = No_label ->
+            get_throw i Ψ = get_throw i Ψ')
+  .
+
+
+  Definition safe_clause Ψ' dec E Ψ Φ : iProp Σ :=
+     match dec with
+    | DE_catch y l =>
+        ∀ vs i f,
+          get_throw y Ψ' vs i -∗
+          EWP v_to_e_list vs ++ [AI_basic (BI_br l)] UNDER f @ E <| Ψ |> {{ Φ }}
+    | DE_catch_ref y l =>
+        ∀ vs i f,
+          get_throw y Ψ' vs i -∗
+          EWP v_to_e_list vs ++ [AI_ref_exn i y; AI_basic (BI_br l)] UNDER f @ E <| Ψ |> {{ Φ }}
+    | DE_catch_all l =>
+        ∀ y vs i f,
+          get_throw y Ψ' vs i -∗
+          EWP v_to_e_list vs ++ [AI_basic (BI_br l)] UNDER f @ E <| Ψ |> {{ Φ }}
+    | DE_catch_all_ref l =>
+        ∀ y vs i f,
+          get_throw y Ψ' vs i -∗
+          EWP v_to_e_list vs ++ [AI_ref_exn i y; AI_basic (BI_br l)] UNDER f @ E <| Ψ |> {{ Φ }}
+    end.
+
+  Lemma firstx_throw_lookup dccs i l:
+    firstx_exception dccs i = Clause_label l ->
+    exists k, dccs !! k = Some (DE_catch i l) \/ dccs !! k = Some (DE_catch_all l).
+  Proof.
+    induction dccs => //=.
+    destruct a => //=.
+    - destruct (eqtype.eq_op i t) eqn:Hit => //.
+      + intros H; inversion H; subst; clear H.
+        apply b2p in Hit as ->.
+        exists 0; by left. 
+      + intros H; apply IHdccs in H as [k Hres].
+        exists (S k) => //.
+    - destruct (eqtype.eq_op i t) eqn:Hit => //.
+      intros H; apply IHdccs in H as [k Hres].
+      exists (S k) => //.
+    - intros H; inversion H; subst. exists 0. by right. 
+  Qed.
+
+   Lemma firstx_throw_lookup_ref dccs i l:
+    firstx_exception dccs i = Clause_label_ref l ->
+    exists k, dccs !! k = Some (DE_catch_ref i l) \/ dccs !! k = Some (DE_catch_all_ref l).
+  Proof.
+    induction dccs => //=.
+    destruct a => //=.
+    - destruct (eqtype.eq_op i t) eqn:Hit => //.
+      intros H; apply IHdccs in H as [k Hres].
+      exists (S k) => //.
+    - destruct (eqtype.eq_op i t) eqn:Hit => //.
+      + intros H; inversion H; subst; clear H.
+        apply b2p in Hit as ->.
+        exists 0; by left. 
+      + intros H; apply IHdccs in H as [k Hres].
+        exists (S k) => //.
+    - intros H; inversion H; subst. exists 0. by right. 
+  Qed.
+   
+
+
+  Lemma thrE_first_instr es vs a i sh :
+    to_eff0 es = Some (thrE vs a i sh) ->
+    exists k, first_instr es = Some (AI_throw_ref_desugared vs a i, k).
+  Proof.
+    remember (S (length_rec es)) as m.
+    assert (length_rec es < m); first by subst; lia.
+    clear Heqm.
+    generalize dependent sh.
+    generalize dependent es.
+    induction m => //.
+    { intros es Hlen; lia. } 
+    intros es Hlen sh.
+    destruct es => //. 
+    unfold to_eff0 => //=.
+    rewrite merge_prepend.
+    destruct (to_val_instr a0) eqn:Ha => //.
+    - destruct v => //=.
+      + unfold to_eff0 in IHm.
+        specialize (IHm es).
+        destruct (merge_values _) => //.
+        * destruct v => //. destruct l => //.
+        * destruct e => //.
+          intros H; inversion H; subst; clear H.
+          edestruct IHm as [k Hes] => //.
+          specialize (length_cons_rec a0 es). lia.
+          unfold first_instr.
+          simpl.
+          unfold first_instr in Hes.
+          rewrite Hes.
+          destruct a0 => //=.
+          destruct b => //=.
+          all: try by eexists.
+          all: simpl in Ha.
+          all: destruct (merge_values _) => //.
+          all: try by destruct v => //.
+          all: try destruct e => //.
+          destruct (exnelts_of_exception_clauses _ _) => //.
+          destruct (suselts_of_continuation_clauses _ _) => //.
+          destruct (swelts_of_continuation_clauses _ _) => //.
+          destruct v => //.
+          destruct i0 => //.
+          destruct (vh_decrease _) => //.
+      + destruct (expr_of_val_not_val _) => //.
+    - destruct e => //.
+      simpl.
+      intros H; inversion H; subst; clear H.
+      destruct a0 => //=.
+      + destruct b => //=.
+      + simpl in Ha. inversion Ha; subst. by eexists.
+      + simpl in Ha.
+        specialize (Logic.eq_refl (to_eff0 l0)) as Heq.
+        unfold to_eff0 in Heq at 2.
+        destruct (merge_values _) => //.
+        destruct v => //.
+        destruct e => //.
+        destruct (exnelts_of_exception_clauses _ _) => //.
+        inversion Ha; subst.
+        apply IHm in Heq as [k Hk].
+        unfold first_instr.
+        unfold first_instr in Hk.
+        simpl.
+        rewrite Hk.
+        by eexists.
+        unfold length_rec in Hlen.
+        unfold length_rec.
+        simpl in Hlen. lia.
+      + simpl in Ha.
+        specialize (Logic.eq_refl (to_eff0 l1)) as Heq.
+        unfold to_eff0 in Heq at 2.
+        destruct (merge_values _) => //.
+        destruct v => //.
+        destruct e => //.
+        destruct suselts_of_continuation_clauses => //.
+        destruct (swelts_of_continuation_clauses _ _) => //.
+        inversion Ha; subst.
+        apply IHm in Heq as [k Hk].
+        unfold first_instr.
+        unfold first_instr in Hk.
+        simpl.
+        rewrite Hk.
+        by eexists.
+        unfold length_rec in Hlen.
+        unfold length_rec.
+        simpl in Hlen. lia.
+      + simpl in Ha.
+        specialize (Logic.eq_refl (to_eff0 l0)) as Heq.
+        unfold to_eff0 in Heq at 2.
+        destruct (merge_values _) => //.
+        destruct v => //.
+        2: destruct e => //.
+        destruct i0 => //.
+        destruct (vh_decrease _) => //. 
+        inversion Ha; subst.
+        apply IHm in Heq as [k Hk].
+        unfold first_instr.
+        unfold first_instr in Hk.
+        simpl.
+        rewrite Hk.
+        by eexists.
+        unfold length_rec in Hlen.
+        unfold length_rec.
+        simpl in Hlen. lia.
+      + simpl in Ha.
+        specialize (Logic.eq_refl (to_eff0 l)) as Heq.
+        unfold to_eff0 in Heq at 2.
+        destruct (merge_values _) => //.
+        destruct v => //.
+        destruct e => //.
+        inversion Ha; subst.
+        apply IHm in Heq as [k Hk].
+        unfold first_instr.
+        unfold first_instr in Hk.
+        simpl.
+        rewrite Hk.
+        by eexists.
+        unfold length_rec in Hlen.
+        unfold length_rec.
+        simpl in Hlen. lia.
+  Qed.
+
+  
+  
+  Lemma ewp_handler hs Ψ Ψ' es f E Φ' Φ:
+    agree_on_uncaptured hs Ψ Ψ' ->
+    ((∀ f, ¬ Φ' trapV f) ∗ EWP es UNDER f @ E <| Ψ' |> {{ Φ' }} ∗
+      (∀ v' f', Φ' v' f' -∗ EWP [AI_handler hs (of_val0 v')] UNDER f' @ E <| Ψ |> {{ Φ }}) ∗
+      ([∗ list] dec ∈ hs, safe_clause Ψ' dec E Ψ Φ)
+      ⊢ EWP [AI_handler hs es] UNDER f @ E <| Ψ |> {{ Φ }})%I.
+  Proof.
+    iLöb as "IH" forall (hs es E Ψ Ψ' Φ Φ' f).
+    iIntros (HΨ) "(Hntrap & Hes & HΦ & Hclauses)".
+    destruct (to_val0 es) eqn:Htv.
+    { iDestruct ewp_value_fupd as "[H _]";
+        last iDestruct ("H" with "Hes") as "Hes".
+      exact Htv. 
+
+      iApply fupd_ewp.
+      unfold to_eff0. simpl.
+      unfold to_val0 in Htv.
+      destruct (merge_values _) => //.
+      destruct v0 => //.
+      iMod "Hes" as "Hes".
+      iDestruct ("HΦ" with "Hes") as "Hres".
+      iModIntro.
+      erewrite of_to_val0 => //.
+    }
+    destruct (to_eff0 es) eqn:Htf.
+    { 
+      destruct e.
+      - iDestruct (ewp_effect_sus with "Hes") as "Hes" ; eauto.
+        remember (Logic.eq_refl (to_eff0 [AI_handler hs es])) as Htf'; clear HeqHtf'.
+        unfold to_eff0 in Htf' at 2.
+        simpl in Htf'.
+        remember Htf as Htf0; clear HeqHtf0.
+        unfold to_eff0 in Htf.
+        destruct (merge_values _) => //.
+        inversion Htf; subst e.
+        simpl in Htf'.
+        iApply ewp_effect_sus; eauto.
+        remember HΨ as HΨ'; clear HeqHΨ'.
+        destruct HΨ as [HΨ _].
+        rewrite -HΨ.
+        iApply (monotonic_prot with "[-Hes] Hes").
+        iIntros (w) "Hw".
+        iNext. iSimpl.
+        unfold to_eff0 in Htf'.
+        simpl in Htf'.
+        destruct (merge_values (List.map _ es)) eqn:HLI => //.
+        destruct v => //.
+        destruct e => //.
+        2:{ destruct (exnelts_of_exception_clauses _ _) => //. } 
+        simpl in Htf' => //.
+        inversion Htf'; subst.
+        iApply "IH".
+        done.
+        iFrame.
+      - destruct i. iDestruct (ewp_effect_sw with "Hes") as "Hes" ; eauto.
+        remember (Logic.eq_refl (to_eff0 [AI_handler hs es])) as Htf'; clear HeqHtf'.
+        unfold to_eff0 in Htf' at 2.
+        simpl in Htf'.
+        remember Htf as Htf0; clear HeqHtf0.
+        unfold to_eff0 in Htf.
+        destruct (merge_values _) => //.
+        inversion Htf; subst e.
+        simpl in Htf'.
+        iApply ewp_effect_sw; eauto.
+        remember HΨ as HΨ'; clear HeqHΨ'.
+        destruct HΨ as (_ & HΨ & _).
+        unfold get_switch2, get_switch1.
+        rewrite -HΨ.
+        iDestruct "Hes" as (?????) "(? & ? & ? & ? & ? & ? & Hes)".
+        iFrame.
+        iApply (monotonic_prot with "[-Hes] Hes").
+        iIntros (w) "Hw".
+        iNext. iSimpl.
+        unfold to_eff0 in Htf'.
+        simpl in Htf'.
+        destruct (merge_values (List.map _ es)) eqn:HLI => //.
+        destruct v => //.
+        destruct e => //.
+        2:{ destruct (exnelts_of_exception_clauses _ _) => //. } 
+        simpl in Htf' => //.
+        inversion Htf'; subst.
+        iApply "IH".
+        done.
+        iFrame.
+      - iDestruct (ewp_effect_thr with "Hes") as "Hes" ; eauto.
+        remember (Logic.eq_refl (to_eff0 [AI_handler hs es])) as Htf'; clear HeqHtf'.
+        unfold to_eff0 in Htf' at 2.
+        simpl in Htf'.
+        remember Htf as Htf0; clear HeqHtf0.
+        unfold to_eff0 in Htf.
+        destruct (merge_values _) => //.
+        inversion Htf; subst e.
+        destruct (exnelts_of_exception_clauses hs i) eqn:Helts.
+        + simpl in Htf'.
+          iApply ewp_effect_thr; eauto.
+          remember HΨ as HΨ'; clear HeqHΨ'.
+          destruct HΨ as (_ & _ & HΨ).
+          rewrite -HΨ. done.
+          eapply exnelts_firstx. exact Helts. 
+        + simpl in Htf'.
+          apply exnelts_of_exception_clauses_None in Helts as Hfirst.
+          iApply ewp_lift_step => //.
+          apply to_val_None_handler => //.
+          iIntros (σ) "Hσ".
+          iApply fupd_mask_intro; first solve_ndisj.
+          iIntros "Hclose".
+          destruct i.
+          destruct (firstx_exception hs (Mk_tagidx n)) eqn:Hfirst' => //. 
+          * apply firstx_throw_lookup in Hfirst' as Hfirst''.
+            destruct Hfirst'' as [k [Hk | Hk]].
+            -- iDestruct (big_sepL_lookup with "Hclauses") as "Hclause".
+               exact Hk.
+               eassert (reduce σ _ [AI_handler hs es] _ _ _).
+               { eapply r_throw_ref.
+                 2: exact Hfirst'. 
+                 apply of_to_eff0 in Htf0.
+                 unfold of_eff0 in Htf0.
+                 rewrite -Htf0.
+                 apply exnfill_to_hfilled. }
+               iSplit.
+               { iPureIntro.
+                 unfold reducible.
+                 eexists _, (_, _) , _, _.
+                 repeat split => //. eauto. }
+               iIntros (es2 σ2 ? Hstep).
+               destruct Hstep as (Hstep & _ & _).
+               edestruct reduce_det. 
+               exact Hstep. exact H.
+               subst.
+               destruct H1 as [(-> & ->) | Habs].
+               ++ iFrame.
+                  iNext. iMod "Hclose". iModIntro.
+                  iApply ("Hclause" with "Hes").
+               ++ apply thrE_first_instr in Htf0 as [k' Htf0].
+                  rewrite first_instr_const in Habs; last by apply v_to_e_is_const_list.
+                  unfold first_instr in Habs.
+                  unfold first_instr in Htf0.
+                  simpl in Habs.
+                  simpl in Htf0.
+                  rewrite Htf0 in Habs.
+                  exfalso.
+                  destruct Habs as [(? & Habs) | (? & ? & ? & Habs & _)] => //.
+            -- iDestruct (big_sepL_lookup with "Hclauses") as "Hclause".
+               exact Hk.
+               eassert (reduce σ _ [AI_handler hs es] _ _ _).
+               { eapply r_throw_ref.
+                 2: exact Hfirst'. 
+                 apply of_to_eff0 in Htf0.
+                 unfold of_eff0 in Htf0.
+                 rewrite -Htf0.
+                 apply exnfill_to_hfilled. }
+               iSplit.
+               { iPureIntro.
+                 unfold reducible.
+                 eexists _, (_, _) , _, _.
+                 repeat split => //. eauto. }
+               iIntros (es2 σ2 ? Hstep).
+               destruct Hstep as (Hstep & _ & _).
+               edestruct reduce_det. 
+               exact Hstep. exact H.
+               subst.
+               destruct H1 as [(-> & ->) | Habs].
+               ++ iFrame.
+                  iNext. iMod "Hclose". iModIntro.
+                  iApply ("Hclause" with "Hes").
+               ++ apply thrE_first_instr in Htf0 as [k' Htf0].
+                  rewrite first_instr_const in Habs; last by apply v_to_e_is_const_list.
+                  unfold first_instr in Habs.
+                  unfold first_instr in Htf0.
+                  simpl in Habs.
+                  simpl in Htf0.
+                  rewrite Htf0 in Habs.
+                  exfalso.
+                  destruct Habs as [(? & Habs) | (? & ? & ? & Habs & _)] => //.
+          * apply firstx_throw_lookup_ref in Hfirst' as Hfirst''.
+            destruct Hfirst'' as [k [Hk | Hk]].
+            -- iDestruct (big_sepL_lookup with "Hclauses") as "Hclause".
+               exact Hk.
+               eassert (reduce σ _ [AI_handler hs es] _ _ _).
+               { eapply r_throw_ref_ref.
+                 2: exact Hfirst'. 
+                 apply of_to_eff0 in Htf0.
+                 unfold of_eff0 in Htf0.
+                 rewrite -Htf0.
+                 apply exnfill_to_hfilled. }
+               iSplit.
+               { iPureIntro.
+                 unfold reducible.
+                 eexists _, (_, _) , _, _.
+                 repeat split => //. eauto. }
+               iIntros (es2 σ2 ? Hstep).
+               destruct Hstep as (Hstep & _ & _).
+               edestruct reduce_det. 
+               exact Hstep. exact H.
+               subst.
+               destruct H1 as [(-> & ->) | Habs].
+               ++ iFrame.
+                  iNext. iMod "Hclose". iModIntro.
+                  iApply ("Hclause" with "Hes").
+               ++ apply thrE_first_instr in Htf0 as [k' Htf0].
+                  rewrite first_instr_const in Habs; last by apply v_to_e_is_const_list.
+                  unfold first_instr in Habs.
+                  unfold first_instr in Htf0.
+                  simpl in Habs.
+                  simpl in Htf0.
+                  rewrite Htf0 in Habs.
+                  exfalso.
+                  destruct Habs as [(? & Habs) | (? & ? & ? & Habs & _)] => //.
+            -- iDestruct (big_sepL_lookup with "Hclauses") as "Hclause".
+               exact Hk.
+               eassert (reduce σ _ [AI_handler hs es] _ _ _).
+               { eapply r_throw_ref_ref.
+                 2: exact Hfirst'. 
+                 apply of_to_eff0 in Htf0.
+                 unfold of_eff0 in Htf0.
+                 rewrite -Htf0.
+                 apply exnfill_to_hfilled. }
+               iSplit.
+               { iPureIntro.
+                 unfold reducible.
+                 eexists _, (_, _) , _, _.
+                 repeat split => //. eauto. }
+               iIntros (es2 σ2 ? Hstep).
+               destruct Hstep as (Hstep & _ & _).
+               edestruct reduce_det. 
+               exact Hstep. exact H.
+               subst.
+               destruct H1 as [(-> & ->) | Habs].
+               ++ iFrame.
+                  iNext. iMod "Hclose". iModIntro.
+                  iApply ("Hclause" with "Hes").
+               ++ apply thrE_first_instr in Htf0 as [k' Htf0].
+                  rewrite first_instr_const in Habs; last by apply v_to_e_is_const_list.
+                  unfold first_instr in Habs.
+                  unfold first_instr in Htf0.
+                  simpl in Habs.
+                  simpl in Htf0.
+                  rewrite Htf0 in Habs.
+                  exfalso.
+                  destruct Habs as [(? & Habs) | (? & ? & ? & Habs & _)] => //. } 
+
+    iApply ewp_unfold.
+    rewrite /ewp_pre /= to_val_None_handler // to_eff_None_handler //.
+    iIntros (σ) "Hσ".
+
+    
+    rewrite ewp_unfold /ewp_pre.
+    rewrite /= Htv Htf.
+    iMod ("Hes" with "Hσ") as "[%Hred Hes]".
+    iModIntro.
+    iSplit.
+    { iPureIntro.
+      destruct Hred as (obs & [es' f'] & σ' & efs & Hred & -> & ->).
+      eassert _ as Hred'.
+      { eapply r_label.
+        exact Hred.
+        instantiate (2 := LH_handler [] hs (LH_base [] []) []).
+        instantiate (2 := 0).
+        rewrite /lfilled /lfill /= app_nil_r //.
+        rewrite /lfilled /lfill /= app_nil_r //. } 
+      eexists [], (_,_), _, [].
+      split; last done.
+      exact Hred'. } 
+    iIntros ([es2 f2] σ2 Hstep).
+    eapply lfilled_prim_step_split_reduce_r in Hstep as Hstep0.
+    2:{ instantiate (1 := []).
+        instantiate (1 := es).
+        instantiate (1 := LH_handler [] hs (LH_base [] []) []).
+        instantiate (1 := 0).
+        unfold lfilled, lfill => //=.
+        repeat rewrite app_nil_r.
+        rewrite eqtype.eq_refl => //. }
+    2:{ destruct Hred as (obs & [es' f'] & σ' & efs & Hred & -> & ->).
+        eexists [], (_,_), _, [].
+        split; last done.
+        exact Hred. } 
+
+    destruct Hstep as [Hstep _].
+    destruct Hstep0 as [(e' & Hstep' & Hfill') | ([lh Htrap] & Hσ)].
+    - iDestruct ("Hes" $! (_,_) _ Hstep') as "Hes".
+      iSimpl.
+      iMod "Hes".
+      repeat iModIntro.
+      repeat iMod "Hes".
+      iModIntro.
+      iDestruct "Hes" as "(Hσ & He')".
+
+      iFrame.
+(*      iIntros "Hf".
+      iDestruct ("He'" with "Hf") as "He'". *)
+      
+      unfold lfilled, lfill in Hfill'.
+      simpl in Hfill'.
+      rewrite app_nil_r in Hfill'.
+      rewrite cat_app app_nil_r in Hfill'.
+      apply b2p in Hfill' as ->.
+      iApply ("IH"). done.
+      iFrame. 
+    - inversion Hσ; subst σ.
+      assert (prim_step (es, f) σ2 [] ([AI_trap], f) σ2 []).
+      { repeat split => //.
+        constructor. econstructor. 2: exact Htrap.
+        intros ->; by simpl in Htv. } 
+      iDestruct ("Hes" $! (_,_) _ H) as "Hes". 
+      iMod "Hes".
+      repeat iModIntro.
+      repeat iMod "Hes".
+      iDestruct "Hes" as "(Hσ & Hes)".
+      (* iDestruct ("Hes" with "Hf") as "Hes". *)
+      iDestruct ewp_value_fupd as "[H _]".
+      instantiate (1 := trapV) => //.
+      instantiate (1 := [AI_trap]) => //.
+      
+      iMod ("H" with "Hes") as "Habs".
+      iDestruct ("Hntrap" with "Habs") as "Habs" => //.
+  Qed. 
+
+  Lemma ewp_try_table f hs hs' es i t1s t2s vs n E Ψ Ψ' Φ Φ':
+    map (desugar_exception_clause (f_inst f)) hs = map Some hs' ->
+    stypes (f_inst f) i = Some (Tf t1s t2s) ->
+    length t1s = length vs ->
+    is_true $ const_list vs ->
+    n = length t2s ->
+    agree_on_uncaptured hs' Ψ Ψ' ->
+    ((∀ f, ¬ Φ' trapV f) ∗ ▷ EWP [AI_label n [] (vs ++ to_e_list es)] UNDER f @ E <| Ψ' |> {{ Φ' }} ∗
+       ▷ (∀ v' f', Φ' v' f' -∗ EWP [AI_handler hs' (of_val0 v')] UNDER f' @ E <| Ψ |> {{ Φ }}) ∗
+       ▷ ([∗ list] dec ∈ hs', safe_clause Ψ' dec E Ψ Φ)
+       ⊢ EWP vs ++ [AI_basic (BI_try_table i hs es)] UNDER f @ E <| Ψ |> {{ Φ }})%I.
+  Proof.
+    iIntros (Hhs Hi Hlen Hvs -> HΨ) "(Hntrap & Hes & HΦ & Hclauses)".
+    iApply ewp_lift_step => //.
+    { rewrite to_val_cat_None2 => //. } 
+    { rewrite to_eff_cat_None2 => //. } 
+    iIntros (σ) "Hσ".
+    iApply fupd_frame_l.
+(*    iDestruct "Hσ" as "(Hfuncs & Hconts & Htags & Htables & Hmems & Hglobals & Hframe & Hrest)".
+    destruct (resources_of_s_cont (s_conts σ)) eqn:Hconts => //. 
+    iDestruct (gen_heap_valid with "Hconts Hcont") as "%Hlook".
+    rewrite gmap_of_list_lookup Nat2N.id in Hlook.
+    rewrite - nth_error_lookup in Hlook.
+    eapply resources_of_s_cont_lookup in Hlook as Hlook'; last exact Hconts. *)
+
+
+    
+    eassert (reduce σ f
+              (vs ++ [AI_basic (BI_try_table i hs es)])
+              σ f
+              _
+           ) as Hred2.
+    { eapply r_try_table => //.
+      exact Hi. done. exact Hhs. } 
+    iSplit.
+    - iPureIntro.
+      unfold language.reducible, language.prim_step => /=.
+      eexists [], (_, _), _, [].
+      repeat split => //.
+      exact Hred2.
+
+    - iApply fupd_mask_intro; first solve_ndisj.
+      iIntros "Hclose !>" (es' σ2 ? HStep).
+      destruct HStep as (H & _).
+      edestruct reduce_det.
+      exact H. exact Hred2.
+      subst.
+      destruct H1 as [[-> ->] | H0].
+      2:{ destruct H0.
+          destruct H0 as (? & Habs).
+          by rewrite first_instr_const in Habs.
+          destruct H0 as (? & ? & ? & Habs & _).
+          rewrite first_instr_const in Habs => //.
+      }
+      iMod "Hclose". iModIntro.
+      iFrame.
+      iApply ewp_handler.
+      exact HΨ.
+      iFrame.
+  Qed.
+
+
+End reasoning_rules.
